theories/examples/ExecFrameworkIntegration.v
@@ -1,6 +1,9 @@
 Require Import String Basics ZArith.
 From ConCert Require Import Misc Notations PCUICtoTemplate
-     PCUICTranslate ExecFrameworkExamples CustomTactics.
+     PCUICTranslate CustomTactics.
+
+From ConCert Require Import Crowdfunding CrowdfundingData SimpleBlockchain Prelude.
+
 Require Import List.
 Require Import PeanoNat.
 Require Import Coq.ssr.ssrbool.
@@ -9,9 +12,10 @@ Require Import Morphisms.
 From SmartContracts Require Import Blockchain Congress Automation.
 
 Import ListNotations.
+
 Open Scope list.
 
-Import AcornBlockchain CrowdfundingContract.
+Import AcornBlockchain CrowdfundingContract CrowdfundingProperties.
 
 Definition expr_to_tc Σ := compose trans (expr_to_term Σ).
 Definition type_to_tc := compose trans type_to_term.
@@ -130,7 +134,7 @@ Section Wrappers.
 
 End Wrappers.
 
-(* Taken from [Congress], because otherwise it is not visible after import *)
+(** Taken from [Congress] *)
 Ltac solve_contract_proper :=
   repeat
     match goal with
@@ -160,7 +164,7 @@ Proof.
   f_equal.
   unfold Receive.receive. destruct x,y;simpl in *.
   inversion H;cbn in *;subst.
-  destruct m0;solve_contract_proper.
+  destruct m;solve_contract_proper.
 Qed.
 
 Definition cf_contract : Contract Setup Msg_coq State_coq :=
@@ -210,7 +214,7 @@ Proof.
       cbn in *. unfold cf_state in *. erewrite contract_states_eq in Hst by eauto.
       cbn in *.
       intro H. eapply IH;eauto. rewrite Current_slot_of_chain_eq in *.
-      inversion e2. erewrite current_slot_eq in H by eauto. easy.
+      inversion e1. erewrite current_slot_eq in H by eauto. easy.
     * (* Deployment *)
       simpl in *.
       rewrite_environment_equiv.
@@ -219,13 +223,13 @@ Proof.
       intro H. destruct ((contract =? to)%address) eqn:Heq.
       ** (* Executing the init method *)
          replace wc with (cf_contract : WeakContract) in * by congruence.
-         cbn in e3. unfold Init.init in *. cbn in e3.
-         unfold Monads.option_bind in e3.
-         destruct (deserialize setup);tryfalse. inversion e3;subst;clear e3.
+         cbn in e2. unfold Init.init in *. cbn in e2.
+         unfold Monads.option_bind in *.
+         destruct (deserialize setup);tryfalse. inversion e2;subst;clear e2.
          rewrite deserialize_serialize in Hst. inversion Hst. subst.
          easy.
       ** rewrite Current_slot_of_chain_eq in *.
-         inversion e4. erewrite current_slot_eq in H by eauto.
+         inversion e3. erewrite current_slot_eq in H by eauto.
          cbn in H.
          eapply IH;eauto.
     * (* Call *)
@@ -235,14 +239,14 @@ Proof.
       ** (* To our contract, runs the [receive] function *)
         subst. cbn in *.
         replace wc with (cf_contract : WeakContract) in * by congruence.
-        cbn in e3.
-        unfold Monads.option_bind in e3.
+        cbn in e2.
+        unfold Monads.option_bind in e2.
         destruct (deserialize prev_state) as [p_local_state | ] eqn:Hps;tryfalse.
         destruct msg as [serialized_msg | ];tryfalse.
         destruct (deserialize serialized_msg) as [msg | ];tryfalse.
         destruct (option_map _ _) eqn:Hopt;tryfalse.
         destruct p as [local_state actions].
-        inversion e3. subst;clear e3.
+        inversion e2;subst;clear e2.
         unfold option_map in Hopt.
         destruct (Receive.receive _ _ _ _) eqn:Hreceive;tryfalse.
         destruct p. inversion Hopt. subst. clear Hopt.
@@ -251,7 +255,7 @@ Proof.
         replace (to =? to)%address with true in * by (symmetry;apply Nat.eqb_refl).
         rewrite deserialize_serialize in Hst. inversion Hst. subst.
         assert (Hprev_consistent: consistent_balance_deadline (Current_slot (of_chain prev)) p_local_state) by
-            (eapply IH;eauto;now rewrite e1).
+            (eapply IH;eauto;now rewrite e0).
         remember (Build_ctx from to _) as ctx.
 
         (* we use one of the functional correctness properties here *)
@@ -270,7 +274,7 @@ Proof.
         cbn in *. unfold set_chain_contract_state in Hst.
         replace ((contract =? to)%address) with false in Hst by (symmetry;now apply Nat.eqb_neq).
         rewrite Current_slot_of_chain_eq in *.
-        inversion e5. erewrite current_slot_eq by eauto.
+        inversion e4. erewrite current_slot_eq by eauto.
         cbn in *.
         eapply IH;eauto.
   + (* Permute queue *)
@@ -313,9 +317,9 @@ Proof.
       destruct_address_eq.
       ** (* Executing the init method *)
          replace wc with (cf_contract : WeakContract) in * by congruence.
-         cbn in e3. unfold Init.init in *. cbn in e3.
-         unfold Monads.option_bind in e3.
-         destruct (deserialize setup);tryfalse. inversion e3;subst;clear e3.
+         cbn in e2. unfold Init.init in *. cbn in e2.
+         unfold Monads.option_bind in e2.
+         destruct (deserialize setup);tryfalse. inversion e2;subst;clear e2.
          rewrite deserialize_serialize in Hst. inversion Hst. subst.
          reflexivity.
       ** eapply IH;eauto.
@@ -326,14 +330,14 @@ Proof.
       ** (* To our contract, runs the [receive] function *)
         subst. cbn in *.
         replace wc with (cf_contract : WeakContract) in * by congruence.
-        cbn in e3.
-        unfold Monads.option_bind in e3.
+        cbn in e2.
+        unfold Monads.option_bind in e2.
         destruct (deserialize prev_state) as [p_local_state | ] eqn:Hps;tryfalse.
         destruct msg as [serialized_msg | ];tryfalse.
         destruct (deserialize serialized_msg) as [msg | ];tryfalse.
         destruct (option_map _ _) eqn:Hopt;tryfalse.
         destruct p as [local_state actions].
-        inversion e3. subst;clear e3.
+        inversion e2;subst;clear e2.
         unfold option_map in Hopt.
         destruct (Receive.receive _ _ _ _) eqn:Hreceive;tryfalse.
         destruct p. inversion Hopt. subst. clear Hopt.
@@ -342,7 +346,7 @@ Proof.
         replace (to =? to)%address with true in * by (symmetry;apply Nat.eqb_refl).
         rewrite deserialize_serialize in Hst. inversion Hst. subst.
         assert (Hprev_consistent: consistent_balance p_local_state) by
-            (eapply IH;eauto;now rewrite e1).
+            (eapply IH;eauto;now rewrite e0).
         remember (Build_ctx from to _) as ctx.
         remember (Build_chain _ _ _ _) as ch.
 
@@ -521,14 +525,14 @@ Proof.
       ** (* To our contract, runs the [receive] function *)
         subst. cbn in *.
         replace wc with (cf_contract : WeakContract) in * by congruence.
-        cbn in e3.
-        unfold Monads.option_bind in e3.
+        cbn in e2.
+        unfold Monads.option_bind in e2.
         destruct (deserialize prev_state) as [p_local_state | ] eqn:Hps;tryfalse.
         destruct msg as [serialized_msg | ];tryfalse.
         destruct (deserialize serialized_msg) as [msg | ];tryfalse.
         destruct (option_map _ _) eqn:Hopt;tryfalse.
         destruct p as [local_state actions].
-        inversion e3. subst;clear e3.
+        inversion e2;subst;clear e2.
         unfold option_map in Hopt.
         destruct (Receive.receive _ _ _ _) eqn:Hreceive;tryfalse.
         destruct p. inversion Hopt. subst. clear Hopt.
@@ -584,9 +588,9 @@ Proof.
   + simpl in *. inversion Hlook;subst.
     unfold is_true in *;repeat rewrite Bool.andb_true_iff in *.
     rewrite <- Zle_is_le_bool in *.
-    assert (sum_map m0 >=0)%Z by now eapply all_non_neg_sum_map. lia.
+    assert (sum_map m >=0)%Z by now eapply all_non_neg_sum_map. lia.
   + specialize_hypotheses.
-    assert (sum_map m0 >=0)%Z by now eapply all_non_neg_sum_map.
+    assert (sum_map m >=0)%Z by now eapply all_non_neg_sum_map.
     rewrite <- Zle_is_le_bool in *.
     lia.
 Qed.
@@ -625,9 +629,9 @@ Proof.
       destruct_address_eq.
       ** (* Executing the init method *)
          replace wc with (cf_contract : WeakContract) in * by congruence.
-         cbn in e3. unfold Init.init in *. cbn in e3.
-         unfold Monads.option_bind in e3.
-         destruct (deserialize setup);tryfalse. inversion e3;subst;clear e3.
+         cbn in e2. unfold Init.init in *. cbn in e2.
+         unfold Monads.option_bind in e2.
+         destruct (deserialize setup);tryfalse. inversion e2;subst;clear e2.
          rewrite deserialize_serialize in Hst. inversion Hst. subst.
          reflexivity.
       ** eapply IH;eauto.
@@ -638,14 +642,14 @@ Proof.
       ** (* To our contract, runs the [receive] function *)
         subst. cbn in *.
         replace wc with (cf_contract : WeakContract) in * by congruence.
-        cbn in e3.
-        unfold Monads.option_bind in e3.
+        cbn in e2.
+        unfold Monads.option_bind in e2.
         destruct (deserialize prev_state) as [p_local_state | ] eqn:Hps;tryfalse.
         destruct msg as [serialized_msg | ];tryfalse.
         destruct (deserialize serialized_msg) as [msg | ];tryfalse.
         destruct (option_map _ _) eqn:Hopt;tryfalse.
         destruct p as [local_state actions].
-        inversion e3. subst;clear e3.
+        inversion e2;subst;clear e2.
         unfold option_map in Hopt.
         destruct (Receive.receive _ _ _ _) eqn:Hreceive;tryfalse.
         destruct p. inversion Hopt. subst. clear Hopt.
@@ -655,7 +659,7 @@ Proof.
         rewrite deserialize_serialize in Hst. inversion Hst. subst.
         assert (Hprev_nneg:
                   map_forallb (Z.leb 0) (donations_coq p_local_state)) by
-            (eapply IH;eauto;now rewrite e1).
+            (eapply IH;eauto;now rewrite e0).
         remember (Build_ctx from to _) as ctx.
         remember (Build_chain _ _ _ _) as ch.
         assert (Ham : (0 <= Ctx_amount ctx)%Z) by (subst ctx;simpl;lia).
@@ -741,7 +745,7 @@ Proof.
       cbn in *.
       intro H. eapply IH;eauto. rewrite Z.compare_lt_iff in *. cbn in *. unfold add_balance in *.
       rewrite queue_prev. simpl.
-      destruct act. inversion e1;subst.
+      destruct act. inversion e0;subst.
       destruct_address_eq;tryfalse;lia.
     * (* Deployment *)
       simpl in *.
@@ -756,9 +760,9 @@ Proof.
          subst;cbn in *;tryfalse.
       ** (* Executing the init method *)
          replace wc with (cf_contract : WeakContract) in * by congruence.
-         cbn in e3. unfold Init.init in *. cbn in e3.
-         unfold Monads.option_bind in e3.
-         destruct (deserialize setup);tryfalse. inversion e3;subst;clear e3.
+         cbn in e2; unfold Init.init in *. cbn in e2.
+         unfold Monads.option_bind in e2.
+         destruct (deserialize setup);tryfalse. inversion e2;subst;clear e2.
          rewrite deserialize_serialize in Hst. inversion Hst. subst.
          cbn in *.
          assert (Htrans : sum_trans to (chain_state_queue prev)%Z = 0%Z).
@@ -787,14 +791,14 @@ Proof.
         (* here goes a lot of boilerplate code *)
          subst. cbn in *.
          replace wc with (cf_contract : WeakContract) in * by congruence.
-         cbn in e3.
-         unfold Monads.option_bind in e3.
+         cbn in e2.
+         unfold Monads.option_bind in e2.
          destruct (deserialize prev_state) as [p_local_state | ] eqn:Hps;tryfalse.
          destruct msg as [serialized_msg | ];tryfalse.
          destruct (deserialize serialized_msg) as [msg | ];tryfalse.
          destruct (option_map _ _) eqn:Hopt;tryfalse.
          destruct p as [local_state actions].
-         inversion e3. subst;clear e3.
+         inversion e2;subst;clear e2.
          unfold option_map in Hopt.
          destruct (Receive.receive _ _ _ _) eqn:Hreceive;tryfalse.
          destruct p. inversion Hopt. subst. clear Hopt.
@@ -805,18 +809,18 @@ Proof.
 
          assert (Hconsistent : consistent_balance p_local_state).
          { (eapply cf_balance_consistent;eauto).
-           constructor. auto. unfold cf_state. now rewrite e1.  }
+           constructor. auto. unfold cf_state. now rewrite e0.  }
 
          assert (Hpos : map_forallb (Z.leb 0) (donations_coq p_local_state)).
          { eapply crowfunding_donations_non_negative;eauto.
-           constructor. auto. unfold cf_state. now rewrite e1. }
+           constructor. auto. unfold cf_state. now rewrite e0. }
          specialize (cf_transfer_cases Hpos Hconsistent Hreceive) as cf_cases.
          destruct cf_cases as [H | [H | H]].
          *** (* donate *)
              destruct H as [H1 H2]. subst. simpl in *. unfold add_balance.
              rewrite queue_new. cbn.
-             specialize (IH eq_refl to e0 Ha p_local_state).
-             rewrite e1 in IH. specialize_hypotheses.
+             specialize (IH eq_refl to e Ha p_local_state).
+             rewrite e0 in IH. specialize_hypotheses.
              rewrite queue_prev in IH. cbn in IH.
              destruct (address_eqb_spec to from).
              **** rewrite <- H1. subst.
@@ -830,8 +834,8 @@ Proof.
              simpl in *. unfold add_balance.
              rewrite queue_new. cbn.
              rewrite address_eq_refl.
-             specialize (IH eq_refl to e0 Ha p_local_state).
-             rewrite e1 in IH. specialize_hypotheses.
+             specialize (IH eq_refl to e Ha p_local_state).
+             rewrite e0 in IH. specialize_hypotheses.
              rewrite queue_prev in IH. cbn in IH.
              destruct (address_eqb_spec to from);subst;lia.
          *** (* claim *)
@@ -839,8 +843,8 @@ Proof.
              simpl in *. unfold add_balance.
              rewrite queue_new. cbn.
              rewrite address_eq_refl.
-             specialize (IH eq_refl to e0 Ha p_local_state).
-             rewrite e1 in IH. specialize_hypotheses.
+             specialize (IH eq_refl to e Ha p_local_state).
+             rewrite e0 in IH. specialize_hypotheses.
              rewrite queue_prev in IH. cbn in IH.
              destruct (address_eqb_spec to from);subst;lia.
       ** (* not to our contract *)
