theories/examples/crowdfunding/Prelude.v
@@ -1,0 +1,210 @@
+(** * Prelude *)
+
+(** Basic definition of data types required for the crowdfunding contract along with notations for developing contract using the deep embedding *)
+
+Require Import String ZArith Basics.
+From ConCert Require Import Ast CustomTactics Notations
+     PCUICTranslate PCUICtoTemplate.
+Require Import List.
+
+From MetaCoq.Template Require Import All.
+
+Import MonadNotation.
+
+Import ListNotations.
+Import BaseTypes.
+Open Scope list.
+
+
+Definition expr_to_tc Σ := compose trans (expr_to_term Σ).
+Definition type_to_tc := compose trans type_to_term.
+Definition global_to_tc := compose trans_minductive_entry trans_global_dec.
+
+(** Our approximation for finite maps. Eventually, will be replaced with the Oak's standard library implementation. We assume that the standard library is available for a contract developer. *)
+Section Maps.
+  Open Scope nat.
+
+  Definition addr_map_acorn :=
+    [\ data "addr_map" =
+          "mnil" [_]
+        | "mcons" [Nat, "Z", "addr_map",_] \].
+
+  Make Inductive (global_to_tc addr_map_acorn).
+
+  Fixpoint lookup_map (m : addr_map) (key : nat) : option Z :=
+    match m with
+    | mnil => None
+    | mcons k v m' =>
+      if (Nat.eqb key k) then Some v else lookup_map m' key
+    end.
+
+  (* Ported from FMapWeaklist of StdLib *)
+  Fixpoint add_map (k : nat) (x : Z) (s : addr_map) : addr_map :=
+  match s with
+   | mnil => mcons k x mnil
+   | mcons k' y l => if Nat.eqb k k' then mcons k x l else mcons k' y (add_map k x l)
+  end.
+
+  Definition inmap_map k m := match lookup_map m k with
+                              | Some _ => true
+                              | None => false
+                              end.
+
+  Lemma lookup_map_add k v m : lookup_map (add_map k v m) k = Some v.
+  Proof.
+    induction m.
+    + simpl. now rewrite PeanoNat.Nat.eqb_refl.
+    + simpl. destruct (k =? n) eqn:Heq.
+      * simpl. now rewrite PeanoNat.Nat.eqb_refl.
+      * simpl. now rewrite Heq.
+  Qed.
+
+  Fixpoint to_list (m : addr_map) : list (nat * Z)%type:=
+    match m with
+    | mnil => nil
+    | mcons k v tl => cons (k,v) (to_list tl)
+    end.
+
+  Fixpoint of_list (l : list (nat * Z)) : addr_map :=
+    match l with
+    | nil => mnil
+    | cons (k,v) tl => mcons k v (of_list tl)
+    end.
+
+  Lemma of_list_to_list m: of_list (to_list m) = m.
+  Proof. induction m;simpl;congruence. Qed.
+
+  Lemma to_list_of_list l: to_list (of_list l) = l.
+  Proof. induction l as [ | x l'];simpl;auto.
+         destruct x. simpl;congruence. Qed.
+
+  Fixpoint map_forallb (p : Z -> bool)(m : addr_map) : bool:=
+    match m with
+    | mnil => true
+    | mcons k v m' => p v && map_forallb p m'
+    end.
+
+  Lemma map_forallb_lookup_map p m k v :
+    map_forallb p m = true ->
+    lookup_map m k = Some v ->
+    p v = true.
+  Proof.
+    revert k v p.
+    induction m;intros;tryfalse;simpl in *.
+    inv_andb H. destruct (_ =? _);auto.
+    * now inversion H0;subst.
+    * easy.
+  Qed.
+
+End Maps.
+
+Notation "a ∈ m" := (inmap_map a m = true) (at level 50).
+Notation "a ∉ m" := (inmap_map a m = false) (at level 50).
+
+(** Generation of string constants using MetaCoq *)
+Fixpoint mkNames (ns : list string) (postfix : string) :=
+  match ns with
+  | [] => tmPrint "Done."
+  | n :: ns' => n' <- tmEval all (n ++ postfix)%string ;;
+                  str <- tmQuote n';;
+                  tmMkDefinition n str;;
+                  mkNames ns' postfix
+  end.
+
+(** Notations for functions on finite maps *)
+
+Definition Map := "addr_map".
+
+Notation "'MNil'" := [| {eConstr "addr_map" "mnil"} |]
+                       (in custom expr at level 0).
+
+Notation "'mfind' a b" :=  [| {eConst "lookup_map"} {a} {b} |]
+        (in custom expr at level 0,
+            a custom expr at level 1,
+            b custom expr at level 1).
+
+Notation "'madd' a b c" :=  [| {eConst "add_map"} {a} {b} {c} |]
+        (in custom expr at level 0,
+            a custom expr at level 1,
+            b custom expr at level 1,
+            c custom expr at level 1).
+
+Notation "'mem' a b" :=  [| {eConst "inmap_map"} {a} {b} |]
+        (in custom expr at level 0,
+            a custom expr at level 1,
+            b custom expr at level 1).
+
+
+  Definition Σ : list global_dec :=
+  [gdInd Unit 0 [("Coq.Init.Datatypes.tt", [])] false;
+     gdInd Bool 0 [("true", []); ("false", [])] false;
+     gdInd Nat 0 [("Z", []); ("Suc", [(None,tyInd Nat)])] false;
+     gdInd "list" 1 [("nil", []); ("cons", [(None,tyRel 0);
+                                              (None,tyApp (tyInd "list") (tyRel 0))])] false;
+     gdInd "prod" 2 [("pair", [(None,tyRel 1);(None,tyRel 0)])] false].
+
+Notation "a + b" := [| {eConst "Coq.ZArith.BinInt.Z.add"} {a} {b} |]
+                      (in custom expr at level 0).
+Notation "a * b" := [| {eConst "Coq.ZArith.BinInt.Z.mul"} {a} {b} |]
+                      (in custom expr at level 0).
+Notation "a - b" := [| {eConst "Coq.ZArith.BinInt.Z.sub"} {a} {b} |]
+                      (in custom expr at level 0).
+Notation "a == b" := [| {eConst "PeanoNat.Nat.eqb"} {a} {b} |]
+                        (in custom expr at level 0).
+Notation "a < b" := [| {eConst "Coq.ZArith.BinInt.Z.ltb"} {a} {b} |]
+                      (in custom expr at level 0).
+Notation "a <= b" := [| {eConst "Coq.ZArith.BinInt.Z.leb"} {a} {b} |]
+                       (in custom expr at level 0).
+Notation "a <n b" := [| {eConst "PeanoNat.Nat.ltb"} {a} {b} |]
+                      (in custom expr at level 0).
+Notation "a <=n b" := [| {eConst "PeanoNat.Nat.leb"} {a} {b} |]
+                      (in custom expr at level 0).
+
+Notation "'Zero'" := (eConstr Nat "Z") ( in custom expr at level 0).
+Notation "'Suc'" := (eConstr Nat "Suc") ( in custom expr at level 0).
+Notation "0" := [| Zero |] ( in custom expr at level 0).
+Notation "1" := [| Suc Zero |] ( in custom expr at level 0).
+
+Notation "'Zero'" := (pConstr "Z" [])
+                (in custom pat at level 0).
+
+Notation "'Suc' x" := (pConstr "Suc" [x])
+                  (in custom pat at level 0,
+                      x constr at level 4).
+
+Notation "a && b" := [| {eConst "andb"} {a} {b} |]
+                       (in custom expr at level 0).
+Notation "~ a" := [| {eConst "negb"} {a} |]
+                      (in custom expr at level 0).
+
+Definition true_name := "true".
+Definition false_name := "false".
+Notation "'True'" := (pConstr true_name []) (in custom pat at level 0).
+Notation "'False'" := (pConstr false_name []) ( in custom pat at level 0).
+
+Notation "'Nil'" := (pConstr "nil" []) (in custom pat at level 0).
+Notation "'Cons' y z" := (pConstr "cons" [y;z])
+                           (in custom pat at level 0,
+                               y constr at level 4,
+                               z constr at level 4).
+
+
+Notation "'True'" := (eConstr Bool true_name) (in custom expr at level 0).
+Notation "'False'" := (eConstr Bool false_name) ( in custom expr at level 0).
+
+Notation "'star'" :=
+  (eConstr Unit "Coq.Init.Datatypes.tt")
+    (in custom expr at level 0).
+
+Definition AcornList : global_dec :=
+  gdInd "list" 1 [("nil", []);("cons", [(None, tyRel 0);(None, (tyApp (tyInd "list") (tyRel 0)))])] false.
+
+Notation List := "list".
+
+Definition Maybe := "option".
+Definition Just := "Some".
+Definition AcornMaybe : global_dec :=
+  gdInd "option" 1 [("Some", [(None, tyRel 0)]);("None", [])] false.
+
+Definition AcornProd : global_dec :=
+  gdInd "prod" 2 [("pair", [(None, tyRel 1); (None, tyRel 0)])] false.
