theories/examples/crowdfunding/SimpleBlockchain.v
@@ -1,0 +1,55 @@
+(** * A simply-typed version of the blockchain execution environment  *)
+(* We develop some blockchain infrastructure relevant for the contract execution. *)
+Require Import String ZArith Basics.
+From ConCert Require Import Ast Notations Prelude PCUICTranslate.
+Require Import List.
+
+From MetaCoq.Template Require Import All.
+
+Import MonadNotation.
+
+Import ListNotations.
+Import BaseTypes.
+Open Scope list.
+
+(** We create a simply-typed records and data types corresponding for
+the actual definitions of [SmartContracts.Blockchain] which are parameterised with [BaseTypes] *)
+
+Module AcornBlockchain.
+  Definition Address := Nat.
+  Definition Money := "Coq.Numbers.BinNums.Z".
+
+
+  Definition SimpleChainAcorn : global_dec :=
+    [\ record "SimpleChain" :=
+       "Build_chain" { "Chain_height" : "nat";
+         "Current_slot" : "nat";
+         "Finalized_height" : "nat";
+         "Account_balance" : Address -> Money } \].
+
+  Notation "'cur_time' a" := [| {eConst "Current_slot"} {a} |]
+                               (in custom expr at level 0).
+
+  Make Inductive (global_to_tc SimpleChainAcorn).
+
+  Definition SimpleContractCallContextAcorn : global_dec :=
+    [\ record "SimpleContractCallContext" :=
+       "Build_ctx" {
+           (* Address sending the funds *)
+           "Ctx_from" : Address;
+           (* Address of the contract being called *)
+           "Ctx_contract_address" : Address;
+           (* Amount of currency passed in call *)
+           "Ctx_amount" : Money} \].
+
+  Make Inductive (global_to_tc SimpleContractCallContextAcorn).
+
+  Definition SimpleActionBodyAcorn : global_dec :=
+    [\ data "SimpleActionBody" =
+          "Act_transfer" [Address, Money,_] \].
+
+  Make Inductive (global_to_tc SimpleActionBodyAcorn).
+
+  Notation SActionBody := "SimpleActionBody".
+
+End AcornBlockchain.
